src/lowparse/LowParse.Spec.Base.fst
@@ -411,6 +411,13 @@ let parser
 : Tot Type0
 = (f: bare_parser t { parser_kind_prop k f } )
 
+let get_parser_kind
+  (#k: parser_kind)
+  (#t: Type0)
+  (p: parser k t)
+: Tot parser_kind
+= k
+
 let parser_kind_prop_intro
   (k: parser_kind)
   (#t: Type0)
